theories/Normalisation.v
@@ -1,145 +1,402 @@
 (** * LogRel.Normalisation: well-typed terms always reduce to a normal form. *)
 From Coq Require Import CRelationClasses.
 From LogRel.AutoSubst Require Import core unscoped Ast Extra.
-From LogRel Require Import Utils BasicAst Notations Context NormalForms Weakening UntypedReduction
-  GenericTyping DeclarativeTyping DeclarativeInstance AlgorithmicTyping.
-From LogRel Require Import LogicalRelation UntypedValues Validity Fundamental.
-From LogRel.LogicalRelation Require Import Escape Neutral Induction ShapeView.
-From LogRel.Substitution Require Import Escape.
+From LogRel Require Import Utils BasicAst Notations LContexts Context NormalForms Weakening UntypedReduction
+  GenericTyping DeclarativeTyping DeclarativeInstance.
+From LogRel Require Import Monad LogicalRelation Validity Fundamental.
+From LogRel.LogicalRelation Require Import Escape Neutral Induction ShapeView Reflexivity Monotonicity.
+From LogRel.Substitution Require Import Escape Poly.
+
+Inductive WN (wl : wfLCon) (t : term) :=
+| WN_ret : forall (wn_val : term)
+                  (wn_red : [ t ⤳* wn_val ]< wl >)
+                  (wn_whnf : whnf wn_val),
+    WN wl t
+| ϝWN {n} {ne : not_in_LCon wl n} :
+  forall (t' : term)
+         (wn_red : [ t ⤳* t' ]< wl >)
+         (wn_whnf : alphane wl n t'),
+  WN (wl ,,l (ne, true)) t ->
+  WN (wl ,,l (ne, false)) t ->
+  WN wl t.
+
+Fixpoint WN_size {wl t} (d : WN wl t) : nat :=
+  match d with
+  | WN_ret _ _ _ _ _ => 0
+  | ϝWN _ _ _ _ _ Ht Hf => S ((WN_size Ht) + (WN_size Hf))
+  end.
+
+Lemma WN_wk : forall wl t (ρ : nat -> nat), WN wl t -> WN wl t⟨ρ⟩.
+Proof.
+  intros * ; induction 1 as [?? r | ].
+  - econstructor 1 with r⟨ρ⟩.
+    + now apply credalg_wk.
+    + now apply whnf_ren.
+  - eapply ϝWN ; [ | | eassumption | eassumption].
+    + now apply credalg_wk.
+    + now apply alphane_ren.
+Qed.
+
+Lemma WN_Ltrans {wl wl' : wfLCon}  {t}: wl' ≤ε wl -> WN wl t -> WN wl' t.
+Proof.
+  intros * f H.
+  revert wl' f ; induction H as [?? r | ] ; intros.
+  + econstructor 1 with r ; tea.
+    now eapply redalg_Ltrans.
+  + destruct (decidInLCon wl' n) as [i | i | notin].
+    * eapply IHWN1.
+      now eapply LCon_le_in_LCon .
+    * eapply IHWN2.
+      now eapply LCon_le_in_LCon .
+    * unshelve eapply ϝWN ; [ | eassumption | | | | eapply IHWN1 | eapply IHWN2].
+      2: eapply redalg_Ltrans ; eassumption.
+      1: eapply alphane_Ltrans ; eassumption.
+      all: now eapply LCon_le_up.
+Defined.
+
+Lemma WN_size_Ltrans {wl wl' : wfLCon} {t} (f: wl' ≤ε wl) (H : WN wl t) :
+  WN_size (WN_Ltrans f H) <= WN_size H.
+Proof.
+  revert wl' f.
+  induction H ; intros.
+  - now constructor.
+  - cbn ; destruct (decidInLCon wl' n) ; cbn.
+    + etransitivity ; [now eapply IHWN1 | ].
+      etransitivity ; [now eapply PeanoNat.Nat.le_succ_diag_r | ].
+      now eapply le_n_S, PeanoNat.Nat.le_add_r.
+    + etransitivity ; [now eapply IHWN2 | ].
+      etransitivity ; [now eapply PeanoNat.Nat.le_succ_diag_r | ].
+      now eapply le_n_S, PeanoNat.Nat.le_add_l.
+    + eapply le_n_S, PeanoNat.Nat.add_le_mono.
+      * now eapply IHWN1.
+      * now eapply IHWN2.
+Qed.
+      
+
+Lemma WN_exp : forall wl t u, [t ⤳* u]< wl > -> WN wl u -> WN wl t.
+Proof.
+  intros wl t u ? ; induction 1 as [?? r | ].
+  - econstructor 1 with r; tea.
+    now etransitivity.
+  - unshelve eapply ϝWN ; [ | eassumption | eassumption | now etransitivity | | eapply IHWN1 | eapply IHWN2].
+    1: eassumption.
+    all: eapply redalg_Ltrans ; eauto.
+    all: now eapply LCon_le_step, wfLCon_le_id.
+Qed.
+
+Lemma WN_red : forall wl t u, [t ⤳* u]< wl > -> WN wl t -> WN wl u.
+Proof.
+  intros wl t u Hred Hyp ; revert u Hred.
+  induction Hyp as [?? r | ] ; intros u Hred.
+  - econstructor 1 with r; tea.
+    now eapply whred_red_det ; eauto.
+  - unshelve eapply ϝWN ; [ | |  | | | eapply IHHyp1 | eapply IHHyp2].
+    3: eassumption.
+    1: eapply whred_red_alphane ; now eauto.
+    all: eapply redalg_Ltrans ; eauto.
+    all: now eapply LCon_le_step, wfLCon_le_id.
+Qed.
+
+Definition drop : wfLCon -> wfLCon.
+Proof.
+  intros [l Hl].
+  destruct l.
+  - exists nil ; assumption.
+  - exists l.
+    now inversion Hl ; subst.
+Defined.
+
+Lemma drop_equal (wl : wfLCon) {n} b {ne : not_in_LCon wl n} :
+  drop (wl ,,l (ne, b)) = wl.
+Proof.
+  destruct wl as [l Hl] ; cbn.
+  reflexivity.
+Qed.
+
+
+Lemma WN_whnf : forall wl t, whnf t -> WN wl t.
+Proof.
+intros; econstructor 1 with t; tea.
+reflexivity.
+Qed.
+
+Lemma WN_isFun : forall wl t, isFun t -> WN wl t.
+Proof.
+intros wl t []; apply WN_whnf; now constructor.
+Qed.
+
+Lemma WN_isPair : forall wl t, isPair t -> WN wl t.
+Proof.
+intros wl t []; apply WN_whnf; now constructor.
+Qed.
+
+Lemma WN_split {wl : wfLCon} {t n} {ne : not_in_LCon wl n} :
+  WN (wl,,l (ne, true)) t ->
+  WN (wl,,l (ne, false)) t ->
+  WN wl t.
+Proof.
+  intros HAt HAf.
+  remember (WN_size HAt + WN_size HAf) as m.
+  apply eq_sym, PeanoNat.Nat.eq_le_incl in Heqm.
+  revert t wl n ne HAt HAf Heqm.
+  induction m ; intros ; cbn in *.
+  - enough (H : WN_size HAt = 0 /\ WN_size HAf = 0).
+    + destruct H ; destruct HAt as [? red | ]; cbn in *.
+      * destruct (alphane_disjunction_redalg red) as [ | [t'' [Ht Hne]]].
+        -- now econstructor 1.
+        -- unshelve econstructor 2 ; try eassumption.
+           now econstructor 1.
+      * now inversion H.
+    + now apply PeanoNat.Nat.eq_add_0, PeanoNat.Nat.le_0_r.
+  - destruct HAt as [? red | k ke ? red ] ; cbn in *.
+    + destruct (alphane_disjunction_redalg red) as [ | [t'' [Ht Hne]]].
+      * now econstructor 1.
+      * unshelve econstructor 2 ; try eassumption.
+        now econstructor 1.
+    + destruct (alphane_disjunction_redalg red) as [ | [t'' [Ht Hne]]].
+      * enough (Hyp : forall (X : not_in_LCon wl k) (b : bool),
+                   WN (wl,,l (X, b)) t).
+        -- unshelve econstructor 2 ; try eassumption.
+           ++ now inversion ke.
+           ++ eapply alphane_backtrans ; try eassumption.
+              now eapply LCon_le_step, wfLCon_le_id.
+           ++ now eapply Hyp.
+           ++ now eapply Hyp.
+        -- intros X b.
+           eapply le_S_n in Heqm.
+           destruct b ; unshelve eapply (IHm _ _ n).
+           ++ abstract (inversion ke ; subst ;
+                        econstructor ; intros ; now eauto).
+           ++ unshelve eapply (WN_Ltrans _ HAt1).
+              eapply LCon_le_in_LCon ; [now eapply LCon_le_up, LCon_le_step, wfLCon_le_id | ].
+              now eapply in_there_l, in_here_l.
+           ++ unshelve eapply (WN_Ltrans _ HAf) ; now eapply LCon_le_up, LCon_le_step, wfLCon_le_id.
+           ++ abstract (inversion ke ; subst ;
+                        econstructor ; intros ; now eauto).
+           ++ unshelve eapply (WN_Ltrans _ HAt2).
+              eapply LCon_le_in_LCon ; [now eapply LCon_le_up, LCon_le_step, wfLCon_le_id | ].
+              now eapply in_there_l, in_here_l.
+           ++ unshelve eapply (WN_Ltrans _ HAf) ; now eapply LCon_le_up, LCon_le_step, wfLCon_le_id.
+           ++ etransitivity ; [ | eassumption].
+              eapply PeanoNat.Nat.add_le_mono ; [ | now apply WN_size_Ltrans].
+              etransitivity ; [ | eapply PeanoNat.Nat.le_add_r ].
+              now apply WN_size_Ltrans.
+           ++ etransitivity ; [ | eassumption].
+              eapply PeanoNat.Nat.add_le_mono ; [ | now apply WN_size_Ltrans].
+              etransitivity ; [ | eapply PeanoNat.Nat.le_add_l ].
+              now apply WN_size_Ltrans.
+      * unshelve econstructor 2 ; [.. | eassumption] ; eauto.
+        unshelve econstructor 2 ; [ .. |  eassumption | eassumption].
+        3: eassumption.
+        assumption.
+Qed.
+  
+Module Nf.
+
+Definition nf : tag.
+Proof.
+constructor.
+Qed.
+
+#[export] Instance WfContextNf : WfContext nf := fun wl Γ => True.
+#[export] Instance WfTypeNf : WfType nf := fun wl Γ A => True.
+#[export] Instance TypingNf : Typing nf := fun wl Γ A t => True.
+#[export] Instance ConvTypeNf : ConvType nf :=
+  fun wl Γ A B => WN wl A × WN wl B.
+#[export] Instance ConvTermNf : ConvTerm nf :=
+  fun wl Γ A t u =>  WN wl t × WN wl u.
+#[export] Instance ConvNeuConvNf : ConvNeuConv nf := fun wl Γ A m n => whne m × whne n.
+#[export] Instance RedTypeNf : RedType nf := fun wl Γ A B => [A ⤳* B ]< wl >.
+#[export] Instance RedTermNf : RedTerm nf := fun wl Γ A t u => [t ⤳* u ]< wl >.
+
+#[export, refine] Instance WfCtxDeclProperties : WfContextProperties (ta := nf) := {}.
+Proof.
+all: try constructor.
+Qed.
+
+#[export, refine] Instance WfTypeDeclProperties : WfTypeProperties (ta := nf) := {}.
+Proof.
+all: try constructor.
+Qed.
+
+#[export, refine] Instance TypingDeclProperties : TypingProperties (ta := nf) := {}.
+Proof.
+all: try constructor.
+Qed.
+
+#[export, refine] Instance ConvTypeDeclProperties : ConvTypeProperties (ta := nf) := {}.
+Proof.
+all: try (intros; split; apply WN_whnf; now constructor).
++ intros * []; now split.
++ intros; split.
+  - intros t u []; now split.
+  - intros t u v [] []; now split.
++ intros * ? []; split; now apply WN_wk.
++ intros * ? ? []; split; now eapply WN_exp.
++ intros * ? [] ; split.
+  all: now eapply WN_Ltrans.
++ intros * [HAt HBt] [HAf HBf] ; split ; now eapply WN_split.
+Qed.
+
+#[export, refine] Instance ConvTermDeclProperties : ConvTermProperties (ta := nf) := {}.
+Proof.
+  all: try (intros; split; apply WN_whnf; now constructor).
+  - intros; split.
+    + intros t u []; now split.
+    + intros t u v [] []; now split.
+  - intros * [] ?; now split.
+  - intros * ? []; split; now apply WN_wk.
+  - intros * ? ? ? ? ? ? []; split; now eapply WN_exp.
+  - intros * ? []; split; now apply WN_whnf, whnf_whne.
+  - intros * ? ? ? Hf ? Hg []; split.
+    + apply WN_isFun; destruct Hf as [|? []]; now constructor.
+    + apply WN_isFun; destruct Hg as [|? []]; now constructor.
+  - intros * ? ? ? Hp ? Hp' ?; split; apply WN_isPair.
+    + destruct Hp as [|? []]; now constructor.
+    + destruct Hp' as [|? []]; now constructor.
+  - intros * ? Hin ; split.
+    + econstructor 1.
+      * econstructor 2 ; [ | reflexivity].
+        now eapply alphaRed.
+      * destruct b ; cbn ; now constructor.
+    + destruct b ; cbn ; econstructor 1 ; try reflexivity.
+      all: now constructor.
+  - intros * f [] ; split.
+    all: now eapply WN_Ltrans.
+  - intros * [] [] ; split ; now eapply WN_split.
+Qed.
+
+#[export, refine] Instance ConvNeuDeclProperties : ConvNeuProperties (ta := nf) := {}.
+Proof.
++ intros; split.
+  - intros t u []; now split.
+  - intros t u v [] []; now split.
++ intros * [] ?; now split.
++ intros * ? []; split; now apply whne_ren.
++ intros * []; assumption.
++ intros; split; constructor.
++ intros * [] ?; split; now constructor.
++ intros * ? ? ? []; split; now constructor.
++ intros * ? []; split; now constructor.
++ intros * ? ? ? []; split; now constructor.
++ intros * []; split ; now constructor.
++ intros * []; split; now constructor.
++ intros * []; split; now constructor.
++ intros * ??????? []; split; now constructor.
++ intros * f [] ; split ; assumption.
++ intros * f [] ; split ; assumption.
+Qed.
+
+#[export, refine] Instance RedTermDeclProperties : RedTermProperties (ta := nf) := {}.
+Proof.
+all: try now (intros; apply redalg_one_step; constructor).
++ intros; now apply credalg_wk.
++ intros; eassumption.
++ now constructor.
++ intros; now apply redalg_app.
++ intros; now apply redalg_natElim.
++ intros; now apply redalg_boolElim.
++ intros * H ; induction H ; [ now eapply redIdAlg | econstructor 2 ; [ | eassumption]].
+  now eapply alphaSubst.
++ intros; now apply redalg_natEmpty.
++ intros; now apply redalg_fst.
++ intros; now apply redalg_snd.
++ intros; now eapply redalg_idElim.
++ intros; assumption.
++ intros; now eapply redIdAlg.
++ intros ; now eapply RedAlgTrans.
++ intros ; now eapply redalg_Ltrans.
+Qed.
+
+#[export, refine] Instance RedTypeDeclProperties : RedTypeProperties (ta := nf) := {}.
+Proof.
+all: try now intros; eassumption.
++ intros; now apply credalg_wk.
++ constructor.
++ intros; now eapply redIdAlg.
++ intros ; now eapply RedAlgTrans.
++ intros ; now eapply redalg_Ltrans.
+Qed.
+
+#[export] Instance DeclarativeTypingProperties : GenericTypingProperties nf _ _ _ _ _ _ _ _ _ _ := {}.
+
+End Nf.
 
 Section Normalisation.
-  Context `{GenericTypingProperties}.
 
-  Theorem typing_nf : WfDeclInductionConcl
-    (fun _ => True)
-    (fun Γ A => Nf[Γ |- A])
-    (fun Γ A t => Nf[Γ |- t : A])
-    (fun Γ A B => Nf[Γ |- A] × Nf[Γ |- B])
-    (fun Γ A t u => Nf[Γ |- t : A] × Nf[Γ |- u : A]).
+  Import Nf.
+
+  Theorem typing_nf {wl} : WfDeclInductionConcl
+    (fun _ _ => True)
+    (fun wl Γ A => True)
+    (fun wl Γ A t => True)
+    (fun wl Γ A B => WN wl A × WN wl B)
+    (fun wl Γ A t u => WN wl t × WN wl u)
+  wl.
   Proof.
     red.
     prod_splitter.
-    all: intros * []%Fundamental.
-    - easy.
-    - now eapply reifyType, reducibleTy.
-    - now eapply reifyTerm, reducibleTm.
-    - split.
-      all: now eapply reifyType, reducibleTy.
-    - split.
-      all: now eapply reifyTerm, reducibleTm.
+    all: intros * H%Fundamental.
+    - constructor.
+    - constructor.
+    - constructor.
+    - destruct H as [? ? ? H].
+      apply escapeEq in H as []; now split.
+    - destruct H as [? ? ? ? H].
+      apply escapeTmEq in H as []; now split.
   Qed.
+
+  Import DeclarativeTypingData.
+
+  Corollary normalisation {wl Γ A t} : [Γ |-[de] t : A]< wl > -> WN wl t.
+  Proof. now intros ?%TermRefl%typing_nf. Qed.
+
+  Corollary type_normalisation {wl Γ A} : [Γ |-[de] A]< wl > -> WN wl A.
+  Proof. now intros ?%TypeRefl%typing_nf. Qed.
 
 End Normalisation.
 
 Import DeclarativeTypingProperties.
 
-Record cored t t' : Prop := { _ : [t' ⇒ t] }.
+Record cored wl t t' : Prop := { _ : [t' ⤳ t]< wl > }.
 
-Theorem typing_SN Γ t :
-  well_typed Γ t ->
-  Acc cored t.
+Lemma cored_acc_backtrans wl wl' t (f : wl' ≤ε wl):
+  Acc (cored wl') t ->
+  Acc (cored wl) t.
 Proof.
-  intros [? Hty].
-  eapply typing_nf in Hty as [? [red wh]].
-  induction red.
-  - econstructor.
-    intros t' [red].
-    exfalso.
-    now eapply whnf_nored.
-  - econstructor.
-    intros t'' [red'].
-    now eapply ored_det in red' as <-.
+  induction 1 as [? H IH] ; econstructor ; intros t' [Hred].
+  eapply IH.
+  econstructor ; eapply red_Ltrans ; eassumption.
 Qed.
 
-Section NeutralConversion.
-  Import AlgorithmicTypingData.
-
-  Lemma ne_conv_conv : forall (Γ : context) (A m n : term),
-    [Γ |-[de] A] ->
-    [Γ |-[al] m ~ n ▹ A] ->
-    [Γ |-[al] m ≅ n : A].
-  Proof.
-    intros * Hty.
-    pose proof (Hty' := Hty).
-    eapply Fundamental in Hty' as [? Hfund%reducibleTy].
-    revert m n.
-    pose (P := (fun Γ A _ _ _ _ => 
-      forall m n, [Γ |-[ al ] m ~ n ▹ A] -> [Γ |-[ al ] m ≅ n : A]) :
-      forall Γ A rEq rTe rTeEq, LR (LogRelRec one) Γ A rEq rTe rTeEq  -> Type).
-    change (P Γ A Hfund.(LRPack.eqTy) Hfund.(LRPack.redTm) Hfund.(LRPack.eqTm) Hfund.(LRAd.adequate)).
-    apply LR_rect.
-    all: subst P ; cbn.
-    - intros.
-      econstructor.
-      1: eapply redty_red; now destruct h as [??? [??]].
-      1-2: reflexivity.
-      econstructor. 
-      2: now constructor.
-      eassumption.
-    - intros * [] ?.
-      econstructor.
-      1: gen_typing.
-      1-2: reflexivity.
-      econstructor.
-      1: eassumption.
-      econstructor; eapply (ty_ne_whne ne).
-    - intros ? ? ΠAd ΠAad IHdom IHcod m n Hconv ; cbn in *.
-      rewrite <- (PiRedTyPack.pack_beta ΠAd ΠAad) in *.
-      remember (PiRedTyPack.pack ΠAd ΠAad) as ΠA in *.
-      clear ΠAd ΠAad HeqΠA.
-      destruct ΠA ; cbn in *.
-      econstructor.
-      1: gen_typing.
-      1-2: reflexivity.
-      econstructor.
-      1-2: econstructor ; now eapply algo_conv_wh in Hconv.
-      eapply convtm_meta_conv.
-      3: reflexivity.
-      1: unshelve eapply IHcod.
-      + exact (tRel var_zero).
-      + apply wk1.
-      + gen_typing.
-      + eapply neuTerm.
-        1: econstructor; reflexivity.
-        2: constructor.
-        all: eapply typing_meta_conv.
-        1,3: now do 2 econstructor ; tea ; boundary.
-        all: now bsimpl.
-      + eapply convne_meta_conv.
-        3: reflexivity.
-        1: econstructor.
-        * replace (tProd _ _) with ((tProd dom cod)⟨↑⟩) by
-            (cbn ; reflexivity).
-          eapply algo_conv_shift.
-          econstructor ; tea.
-          1: now gen_typing.
-          econstructor.
-        * eapply convtm_meta_conv.
-          1: unshelve eapply IHdom.
-          -- now eapply wk1.
-          -- gen_typing.
-          -- eapply convne_meta_conv.
-             1: do 2 econstructor.
-             2: reflexivity.
-             now bsimpl.
-          -- now bsimpl.
-          -- reflexivity.
-        * now bsimpl.
-      + bsimpl.
-        rewrite scons_eta'.
-        now bsimpl.
-  - intros Δ B NB **; destruct NB.
-    econstructor.
-    + now eapply redtywf_red.
-    + reflexivity.
-    + reflexivity.
-    + econstructor; [eassumption|constructor].
-  - intros Δ B NB **; destruct NB.
-    econstructor.
-    + now eapply redtywf_red.
-    + reflexivity.
-    + reflexivity.
-    + econstructor; [eassumption|constructor].
+Theorem typing_SN wl Γ t :
+  well_formed wl Γ t ->
+  Acc (cored wl) t.
+Proof.
+  intros [[] Hty].
+  all: first [apply TypeRefl in Hty|apply TermRefl in Hty].
+  all: eapply typing_nf in Hty as [? _].
+  all: induction w as [?? wh red | ].
+  - all: induction red.
+    + econstructor.
+      intros t' [red].
+      exfalso.
+      eapply whnf_nored ; tea.
+    + econstructor.
+      intros t'' [red'].
+      eapply ored_det in red' as <-; [|exact o].
+      apply IHred; tea.
+  - clear IHw2 w1 w2 wn_red wn_whnf.
+    eapply cored_acc_backtrans ; try eassumption.
+    now eapply LCon_le_step, wfLCon_le_id.
+  - induction red.
+    + econstructor ; intros t' [Hred ].
+      exfalso.
+      now eapply whnf_nored.
+    + econstructor.
+      intros t'' [red'].
+      eapply ored_det in red' as <-; [|exact o].
+      apply IHred; now tea.
+  - eapply cored_acc_backtrans ; try eassumption.
+    now eapply LCon_le_step, wfLCon_le_id.
 Qed.
-
-End NeutralConversion.
